compiler/dafny/semantics/dafny_compilerProofScript.sml
@@ -11,289 +11,13 @@ open dafny_to_cakemlProofTheory
 open dafny_compilerTheory
 open mlstringTheory  (* isPrefix *)
 
+open danielTheory
+
 val _ = new_theory "dafny_compilerProof";
 val _ = set_grammar_ancestry
           ["dafny_semanticPrimitives", "dafny_freshen", "dafny_freshenProof",
            "dafny_to_cakeml", "dafny_to_cakemlProof", "dafny_compiler",
-           "mlstring"];
-
-(* TODO Upstream? *)
-Triviality UNZIP_LENGTH:
-  ∀xs ys zs. UNZIP xs = (ys, zs) ⇒ LENGTH ys = LENGTH zs
-Proof
-  Induct \\ gvs []
-QED
-
-(* TODO Upstream? *)
-Triviality UNZIP_EQ_NIL:
-  (UNZIP l = (xs, []) ⇔ l = [] ∧ xs = []) ∧
-  (UNZIP l = ([], ys) ⇔ l = [] ∧ ys = [])
-Proof
-  Cases_on ‘l’ \\ gvs []
-QED
-
-(* TODO Upstream? *) (* by Magnus *)
-Theorem exists_mlstring:
-  (∃x:mlstring. P x) ⇔ (∃s. P (strlit s))
-Proof
-  eq_tac \\ rw []
-  >- (Cases_on ‘x’ \\ gvs [] \\ pop_assum $ irule_at Any)
-  \\ pop_assum $ irule_at Any
-QED
-
-(* TODO Upstream? *)
-Theorem isprefix_strcat:
-  ∀s₁ s₂. isPrefix s₁ s₂ = ∃s₃. s₂ = s₁ ^ s₃
-Proof
-  rpt gen_tac
-  \\ gvs [isprefix_thm, strcat_thm, isPREFIX_STRCAT, exists_mlstring,
-          implode_def]
-  \\ Cases_on ‘s₂’ \\ simp []
-QED
-
-(* TODO Move is_fresh properties to to separate file? *)
-
-(* ** *)
-(* TODO Already exists in freshenProof; make it Theorem *)
-Triviality map_add_fresh_exists:
-  ∀m cnt ns cnt' m'.
-    map_add_fresh m cnt ns = (cnt', m') ⇒
-    ∃m₁. m' = m₁ ++ m ∧ MAP FST m₁ = REVERSE ns
-Proof
-  Induct_on ‘ns’ \\ rpt strip_tac
-  \\ gvs [map_add_fresh_def, add_fresh_def]
-  \\ last_x_assum drule_all \\ rpt strip_tac \\ gvs []
-QED
-
-(* TODO Already exists in freshenProof; make it Theorem *)
-Triviality lookup_append_eq:
-  ∀n m₁ m₀.
-    MEM n (MAP FST m₁) ⇒ lookup (m₁ ++ m₀) n = lookup m₁ n
-Proof
-  rpt strip_tac
-  \\ gvs [lookup_def, ALOOKUP_APPEND]
-  \\ Cases_on ‘ALOOKUP m₁ n’
-  \\ gvs [ALOOKUP_NONE]
-QED
-
-(* TODO Already exists in freshenProof; make it Theorem *)
-Triviality freshen_rhs_exp_len_eq:
-  ∀m cnt rhss cnt' rhss'.
-    freshen_rhs_exps m cnt rhss = (cnt', rhss') ⇒
-    LENGTH rhss' = LENGTH rhss
-Proof
-  Induct_on ‘rhss’ \\ rpt strip_tac
-  \\ gvs [freshen_rhs_exps_def]
-  \\ rpt (pairarg_tac \\ gvs[])
-  \\ res_tac
-QED
-
-(* TODO Already exists in freshenProof; make it Theorem *)
-Triviality freshen_lhs_exp_len_eq:
-  ∀m cnt lhss cnt' lhss'.
-    freshen_lhs_exps m cnt lhss = (cnt', lhss') ⇒
-    LENGTH lhss' = LENGTH lhss
-Proof
-  Induct_on ‘lhss’ \\ rpt strip_tac
-  \\ gvs [freshen_lhs_exps_def]
-  \\ rpt (pairarg_tac \\ gvs[])
-  \\ res_tac
-QED
-
-(* ** *)
-
-Triviality map_add_fresh_every_is_fresh:
-  ∀ns m cnt cnt' m'.
-    map_add_fresh m cnt ns = (cnt', m') ∧
-    ALL_DISTINCT ns ⇒
-    EVERY (λn. is_fresh n) (MAP (lookup m') ns)
-Proof
-  Induct \\ simp []
-  \\ qx_gen_tac ‘n’ \\ rpt strip_tac
-  >-
-   (drule map_add_fresh_exists
-    \\ rpt strip_tac \\ gvs []
-    \\ ‘MEM n (MAP FST m₁)’ by gvs []
-    \\ drule lookup_append_eq \\ simp []
-    \\ disch_then kall_tac
-    \\ simp [lookup_def]
-    \\ CASE_TAC
-    >- (gvs [ALOOKUP_NONE])
-    \\ simp [is_fresh_def, isprefix_strcat])
-  \\ gvs [map_add_fresh_def, add_fresh_def]
-  \\ last_assum irule
-  \\ last_assum $ irule_at Any
-QED
-
-Triviality add_fresh_is_fresh:
-  add_fresh m cnt v = (cnt', m') ⇒ is_fresh (lookup m' v)
-Proof
-  disch_tac \\ gvs [add_fresh_def, lookup_def, is_fresh_def, isprefix_strcat]
-QED
-
-Definition get_param_names_def[simp]:
-  get_param_names (Method _ ins _ _ _ _ outs _ _) =
-    MAP FST ins ++ MAP FST outs ∧
-  get_param_names (Function _ ins _ _ _ _ _) = MAP FST ins
-End
-
-Triviality freshen_exp_is_fresh:
-  (∀m cnt e cnt' e'.
-     freshen_exp m cnt e = (cnt', e') ⇒ is_fresh_exp e') ∧
-  (∀m cnt es cnt' es'.
-     freshen_exps m cnt es = (cnt', es') ⇒
-     EVERY (λe. is_fresh_exp e) es')
-Proof
-  ho_match_mp_tac freshen_exp_ind
-  \\ rpt strip_tac
-  >~ [‘Var v’] >-
-   (gvs [freshen_exp_def]
-    \\ rpt (pairarg_tac \\ gvs [])
-    \\ gvs [is_fresh_def, lookup_def]
-    \\ CASE_TAC >- (simp [isprefix_thm])
-    \\ simp [isprefix_strcat])
-  >~ [‘Forall (v,ty) e’] >-
-   (gvs [freshen_exp_def]
-    \\ rpt (pairarg_tac \\ gvs [])
-    \\ imp_res_tac add_fresh_is_fresh)
-  \\ gvs [freshen_exp_def]
-  \\ rpt (pairarg_tac \\ gvs [])
-QED
-
-Triviality freshen_lhs_exp_is_fresh:
-  freshen_lhs_exp m cnt lhs = (cnt', lhs') ⇒ is_fresh_lhs_exp lhs'
-Proof
-  Cases_on ‘lhs’
-  >~ [‘VarLhs var’] >-
-   (rpt strip_tac
-    \\ gvs [is_fresh_lhs_exp, freshen_lhs_exp_def, lookup_def, is_fresh_def]
-    \\ CASE_TAC >- simp [isprefix_thm]
-    \\ simp [isprefix_strcat])
-  >~ [‘ArrSelLhs arr idx’] >-
-   (rpt strip_tac
-    \\ gvs [freshen_lhs_exp_def]
-    \\ rpt (pairarg_tac \\ gvs [])
-    \\ imp_res_tac (cj 1 freshen_exp_is_fresh) \\ simp [])
-QED
-
-Triviality freshen_lhs_exps_is_fresh:
-  ∀lhss m cnt cnt' lhss'.
-    freshen_lhs_exps m cnt lhss = (cnt', lhss') ⇒
-    EVERY (λe. is_fresh_lhs_exp e) lhss'
-Proof
-  Induct \\ simp [freshen_lhs_exps_def]
-  \\ rpt strip_tac
-  \\ rpt (pairarg_tac \\ gvs [])
-  \\ imp_res_tac freshen_lhs_exp_is_fresh \\ simp []
-  \\ res_tac
-QED
-
-Triviality freshen_rhs_exp_is_fresh:
-  freshen_rhs_exp m cnt rhs = (cnt', rhs') ⇒ is_fresh_rhs_exp rhs'
-Proof
-  Cases_on ‘rhs’
-  >~ [‘ExpRhs e’] >-
-   (simp [freshen_rhs_exp_def]
-    \\ rpt strip_tac
-    \\ rpt (pairarg_tac \\ gvs [])
-    \\ imp_res_tac (cj 1 freshen_exp_is_fresh))
-  >~ [‘ArrAlloc len init’] >-
-   (simp [freshen_rhs_exp_def]
-    \\ rpt strip_tac
-    \\ rpt (pairarg_tac \\ gvs [])
-    \\ imp_res_tac (cj 1 freshen_exp_is_fresh) \\ simp [])
-QED
-
-Triviality freshen_rhs_exps_is_fresh:
-  ∀rhss m cnt cnt' rhss'.
-    freshen_rhs_exps m cnt rhss = (cnt', rhss') ⇒
-    EVERY (λe. is_fresh_rhs_exp e) rhss'
-Proof
-  Induct \\ simp [freshen_rhs_exps_def]
-  \\ rpt strip_tac
-  \\ rpt (pairarg_tac \\ gvs [])
-  \\ imp_res_tac freshen_rhs_exp_is_fresh \\ simp []
-  \\ res_tac
-QED
-
-Triviality freshen_stmt_is_fresh:
-  ∀stmt m cnt cnt' stmt'.
-    freshen_stmt m cnt stmt = (cnt', stmt') ⇒ is_fresh_stmt stmt'
-Proof
-  Induct \\ rpt gen_tac
-  >~ [‘MetCall lhss name args’] >-
-   (simp [freshen_stmt_def]
-    \\ rpt strip_tac
-    \\ rpt (pairarg_tac \\ gvs [])
-    \\ imp_res_tac freshen_lhs_exps_is_fresh \\ simp []
-    \\ imp_res_tac (cj 2 freshen_exp_is_fresh))
-  >~ [‘Dec local scope’] >-
-   (simp [freshen_stmt_def]
-    \\ rpt strip_tac
-    \\ rpt (pairarg_tac \\ gvs [])
-    \\ imp_res_tac add_fresh_is_fresh \\ simp []
-    \\ res_tac)
-  >~ [‘Then stmt₀ stmt₁’] >-
-   (simp [freshen_stmt_def]
-    \\ rpt strip_tac
-    \\ rpt (pairarg_tac \\ gvs [])
-    \\ res_tac \\ simp [])
-  >~ [‘If tst thn els’] >-
-   (simp [freshen_stmt_def]
-    \\ rpt strip_tac
-    \\ rpt (pairarg_tac \\ gvs [])
-    \\ imp_res_tac (cj 1 freshen_exp_is_fresh) \\ simp []
-    \\ res_tac \\ simp [])
-  >~ [‘Assign ass’] >-
-   (simp [freshen_stmt_def]
-    \\ rpt strip_tac
-    \\ rpt (pairarg_tac \\ gvs [])
-    \\ EVERY (map imp_res_tac
-               [freshen_rhs_exp_len_eq, freshen_lhs_exp_len_eq,
-                freshen_rhs_exps_is_fresh, freshen_lhs_exps_is_fresh])
-    \\ simp [MAP_ZIP])
-  >~ [‘While grd invs decrs mods body’] >-
-   (simp [freshen_stmt_def]
-    \\ rpt strip_tac
-    \\ rpt (pairarg_tac \\ gvs [])
-    \\ imp_res_tac freshen_exp_is_fresh
-    \\ simp [] \\ res_tac)
-  >~ [‘Print e ty’] >-
-   (simp [freshen_stmt_def]
-    \\ rpt strip_tac
-    \\ rpt (pairarg_tac \\ gvs [])
-    \\ imp_res_tac freshen_exp_is_fresh)
-  >~ [‘Assert e’] >-
-   (simp [freshen_stmt_def]
-    \\ rpt strip_tac
-    \\ rpt (pairarg_tac \\ gvs [])
-    \\ imp_res_tac freshen_exp_is_fresh)
-  (* Return, Skip *)
-  \\ simp [freshen_stmt_def]
-QED
-
-Triviality freshen_member_is_fresh:
-  ALL_DISTINCT (get_param_names member) ⇒
-  is_fresh_member (freshen_member member)
-Proof
-  disch_tac
-  \\ namedCases_on ‘member’
-       ["name ins reqs ens rds decrs outs mods body",
-        "name ins res_t reqs rds decrs body"]
-  \\ gvs [freshen_member_def]
-  \\ rpt (pairarg_tac \\ gvs [])
-  \\ EVERY (map imp_res_tac
-                [freshen_exp_is_fresh, UNZIP_LENGTH,
-                 map_add_fresh_every_is_fresh, freshen_stmt_is_fresh])
-  \\ gvs [MAP_ZIP, UNZIP_MAP, ALL_DISTINCT_APPEND]
-QED
-
-
-
-
-
-
-(* *** *)
+           "mlstring", "daniel"];
 
 Triviality has_main_freshen:
   has_main (Program (MAP freshen_member members)) =
@@ -325,6 +49,15 @@ Proof
   \\ irule freshen_member_is_fresh \\ simp []
 QED
 
+Triviality map_freshen_member_no_shadow_method:
+  EVERY (λmember. ALL_DISTINCT (get_param_names member)) members ⇒
+  EVERY no_shadow_method (MAP freshen_member members)
+Proof
+  Induct_on ‘members’ \\ simp []
+  \\ rpt strip_tac
+  \\ irule no_shadow_method_freshen_member \\ simp []
+QED
+
 Theorem correct_compile:
   ∀dfy_ck prog s' r_dfy cml_decs env_cml (t: 'ffi cml_state).
     evaluate_program dfy_ck T prog = (s', r_dfy) ∧
@@ -345,9 +78,8 @@ Proof
   \\ namedCases_on ‘prog’ ["members"]
   \\ simp [valid_prog_def, freshen_program_def, has_main_freshen]
   \\ irule_at (Pos hd) map_freshen_member_is_fresh
-  \\ conj_tac >- (fs [valid_members_def])
-
-  \\ cheat
+  \\ irule_at (Pos last) map_freshen_member_no_shadow_method
+  \\ fs [valid_members_def]
 QED
 
 
